CTree/EffectAlgebra.lean
@@ -1,7 +1,7 @@
 import CTree.Monad
 
-abbrev parametricFun (E : Type u → Type v1) (F : Type u → Type v2) :=
-  ∀ {α : Type u}, E α → F α
+abbrev parametricFun (E : Type u → Type v1) (F : Type (max (max (u + 1) w1) w2) → Type v2) :=
+  ∀ {α : Type u}, E α → F (ULift (ULift.{w1, _} (PLift α)))
 infixr:50 " ⟹ "=> parametricFun
 
 inductive SumE (ε1 ε2 : Type u → Type v) : Type u → Type v
@@ -27,46 +27,21 @@ namespace CTree
           | .inl l => .inr <| tau' <| rec <| .bindS (step l)
           | .inr r => .inl <| ret r
         | ⟨.tau, c⟩ => .inr <| tau' <| rec <| .bindS <| c _fin0
-        | ⟨.vis _ e, k⟩ => .inr <| vis' e <| fun a => rec <| .bindS <| k (ULift.up a)
+        | ⟨.vis _ e, k⟩ => .inr <| vis' e <| fun a => rec <| .bindS <| k (PLift.up a)
         | ⟨.zero, _⟩ => .inr <| zero'
         | ⟨.choice, cts⟩ => .inr <| choice' (rec <| .bindS <| cts _fin0) (rec <| .bindS <| cts _fin1)
       | .iterS i => .inr <| tau' <| rec <| .bindS (step i)
     ) (.iterS i)
 
-  def interp' {ε1 ε2 ρ} (handler : ε1 ⟹ CTree ε2) (t : CTree ε1 ρ) : CTree ε2 ρ :=
+  def interp' {ε1 : Type u1 → Type v1} {ε2 : Type u2 → Type v2}
+    (handler : ∀ {α : Type u1}, ε1 α → CTree ε2 (ULift (ULift.{v1, _} (PLift α))))
+    {ρ : Type v3} (t : CTree ε1 ρ) : CTree ε2 ρ :=
     iter (fun t =>
       t.matchOn
       (fun v => ret <| .inr v)
       (fun t => ret <| .inl t)
-      (fun e k => handler e >>= fun a => ret <| .inl <| k a)
+      (fun e k => handler e >>= fun a => ret <| .inl <| k a.down.down.down)
       zero
       (fun c1 c2 => ret <| .inl <| c1 ⊕ c2)
     ) t
-
-  inductive interpState {ε1 ε2 ρ}
-  | iterS (i : CTree ε1 ρ)
-  | bindS (t : CTree ε2 α) (tk : α → CTree ε1 ρ)
-
-  /--
-    Interpret `CTree`s of one effect type into a `CTree` with a different effect type.
-  -/
-  def interp {ε1 ε2 ρ} (handler : ε1 ⟹ CTree ε2) (t : CTree ε1 ρ) : CTree ε2 ρ :=
-    .corec' (fun rec (s : interpState) =>
-      match s with
-      | .bindS t tk =>
-        match t.dest with
-        | ⟨.ret v, _⟩ => .inr <| tau' <| rec <| .iterS (tk v)
-        | ⟨.tau, c⟩ => .inr <| tau' <| rec <| .bindS (c _fin0) tk
-        | ⟨.vis _ e, k⟩ => .inr <| vis' e <| fun a => rec <| .bindS (k (ULift.up a)) tk
-        | ⟨.zero, _⟩ => .inr <| zero'
-        | ⟨.choice, cts⟩ => .inr <| choice' (rec <| .bindS (cts _fin0) tk) (rec <| .bindS (cts _fin1) tk)
-      | .iterS t =>
-        match t.dest with
-        | ⟨.ret v, _⟩ => .inl <| ret v
-        | ⟨.tau, c⟩ => .inr <| tau' <| rec <| .iterS (c _fin0)
-        | ⟨.vis _ e, k⟩ => .inr <| tau' <| rec <| .bindS (handler e) (fun a => k <| .up a)
-        | ⟨.zero, _⟩ => .inr <| zero'
-        | ⟨.choice, cts⟩ => .inr <| choice' (rec <| .iterS (cts _fin0)) (rec <| .iterS (cts _fin1))
-    ) (.iterS t)
-
 end CTree
